% Problem 1.1
\begin{homeworkProblem}
% Problem 1.1 a)
\begin{homeworkSection}{a)}
\begin{align}
   D^{\dagger}(\alpha) a D(\alpha) &=
   e^{A} a e^{-A} \text{\quad where $ A = \bar{\alpha}a - \alpha a^{\dagger}$}
   \intertext{By way of the BCH lemma this can be expressed as}
   &= a + [A,a] + \frac{1}{2}[A,[A,a]] + \ldots
\end{align}

\begin{align}
   [A,a] &= [\bar{\alpha}a - \alpha a^{\dagger},a] \\
         &= -\alpha [a^{\dagger}, a] \\
         &= \alpha \\
   [A,[A,a]] &= [A,\alpha] = 0
\end{align}

So,
\[
   D^{\dagger}(\alpha) a D(\alpha) = a + \alpha
\]


\end{homeworkSection}

% Problem 1.1 b)
\begin{homeworkSection}{b)}
\begin{align}
   S^{\dagger}(\xi) a S(\xi) &= e^{A}ae^{-A} \text{\quad where $ A = \frac{\xi}{2}
   (a^{\dagger})^{2} - \frac{\bar{\xi}}{2} a^{2}$.}
   \intertext{By way of the BCH lemma this can be expressed as}
   &= a + [A,a] + \frac{1}{2}[A,[A,a]] + \frac{1}{3!}[A,[A,[A,a]]] +
\frac{1}{4!}[A,[A,[A,[A,a]]]] + \ldots
\end{align}

% Define operator A
\newcommand\Aop{
   \ensuremath{
      \frac{\xi}{2} (a^{\dagger})^{2} - \frac{\bar{\xi}}{2} a^{2}
   }
}

\begin{align}
   [A,a] &= \left[\Aop,a\right] \\
         &= \frac{\xi}{2}[a^{\dagger} a^{\dagger},a]
   \intertext{Using $ [AB,C] = A[B,C] + [A,C]B $}
   &= \frac{\xi}{2}\left(a^{\dagger}[a^{\dagger},a] + [a^{\dagger},a]a^{\dagger}\right)\\
   &= -\xi a^{\dagger} \text{\quad since $ [a,a^{\dagger}] = 1 $}
\end{align}

\begin{align}
   [A,[A,a]] &= \left[\Aop,-\xi a^{\dagger}\right] \\
             &= \frac{\left| \xi \right|^2}{2} \left[ a^{2}, a^{\dagger} \right]
   \\
   &= \frac{\left| \xi \right|^2}{2}
   \left(
      a\left[ a, a^{\dagger} \right] + \left[ a, a^{\dagger} \right]a
   \right) \\
   &= \left| \xi \right|^2 a
\end{align}

\begin{align}
   [A,[A,[A,a]]] &= \left[ \Aop, \left| \xi \right|^{2} a \right] \\
                &= \frac{\xi \left| \xi \right|^{2}}{2}
   [\left( a^{\dagger} \right)^{2}, a] \\
   &= -\xi \left| \xi \right|^{2} a^{\dagger}
\end{align}

\begin{align}
   [A,[A,[A,[A,a]]]] &= \left[ \Aop, -\xi \left| \xi \right|^{2} a^{\dagger}
   \right] \\
   &= \frac{\left| \xi \right|^{4}}{2}\left[a^{2}, a^{\dagger}\right] \\
   &= \left| \xi \right|^{4} a
\end{align}

At this point it's easy to recognize a pattern emerging. Each odd term in the
expansion only includes $ a $ and increasing even powers of $ \left| \xi \right|^{n}
$. Each even term in the expansion only includes $ a^{\dagger} $ and increasing
even powers of $ -\xi \left| \xi \right|^{n} $. So, we can write

\begin{align}
   S^{\dagger}(\xi)aS(\dagger) &=
   \sum^{\infty}_{i=0} \frac{\left| \xi \right|^{2n}}{(2n)!} a -
   \sum^{\infty}_{i=0} \frac{\xi \left| \xi \right|^{2n}}{(2n+1)!} a^{\dagger}
   \\
   &=
   \sum^{\infty}_{i=0} \frac{\left| \xi \right|^{2n}}{(2n)!} a -
   \sum^{\infty}_{i=0} \frac{\xi \left| \xi \right|^{2n+1}}{\left| \xi
   \right|(2n+1)!} a^{\dagger} \\
   &= \cosh(r)a - \sinh(r)e^{i \phi}a^{\dagger}
\end{align}

\end{homeworkSection}
\end{homeworkProblem}
