\begin{homeworkProblem}

\textbf{Problem Description.}

% Problem 1.1 a)
\begin{homeworkSection}{a)}
\begin{align}
   D^{\dagger}(\alpha) a D(\alpha) &=
   e^{A} a e^{-A} \text{\quad where $ A = \bar{\alpha}a - \alpha a^{\dagger}$}
   \intertext{By way of the BCH lemma this can be expressed as}
   &= a + [A,a] + \frac{1}{2}[A,[A,a]] + \ldots
\end{align}

\begin{align}
   [A,a] &= [\bar{\alpha}a - \alpha a^{\dagger},a] \\
         &= -\alpha [a^{\dagger}, a] \\
         &= \alpha \\
   [A,[A,a]] &= [A,\alpha] = 0
\end{align}

So,
\[
   D^{\dagger}(\alpha) a D(\alpha) &= a + \alpha
\]


\end{homeworkSection}

% Problem 1.1 b)
\begin{homeworkSection}{b)}
\end{homeworkSection}
\end{homeworkProblem}
