% Problem 1.2
\begin{homeworkProblem}

\textbf{Problem Description.}

\begin{homeworkSection}{}
   \begin{align}
      [a, D(\alpha)] &= \alpha D(\alpha) \\
                     &=
      \left[
         a, \exp\left(\frac{-\left| \alpha \right|^{2}}{2}\right)
         e^{\alpha a^{\dagger}}
         e^{-\bar{\alpha}a}
      \right] \\
      &=
       \exp\left(\frac{-\left| \alpha \right|^{2}}{2}\right)
       \left[
         a,
         e^{\alpha a^{\dagger}}
         e^{-\bar{\alpha}a}
      \right]
      \intertext{Identifying $ B = e^{\alpha a^{\dagger}} $ and $ C =
      e^{-\bar{\alpha}a} $}
      &=
       \exp\left(\frac{-\left| \alpha \right|^{2}}{2}\right)
       \left[ a, B C \right] \\
       &= \exp\left(\frac{-\left| \alpha \right|^{2}}{2}\right)
       \left(\left[ a,B \right]C + B[a,C]\right) \\
       &= \exp\left(\frac{-\left| \alpha \right|^{2}}{2}\right)
       \left(\left[ a,e^{\alpha a^{\dagger}} \right] e^{-\bar{\alpha}a} +
       \left[ a, e^{-\bar{\alpha}a}\right] e^{\alpha a^{\dagger}}\right)
       \intertext{The first commutator can be evaluated by expanding the
       exponential into in an infinite series and considering the infinite
    series of commutators. The second commutator evaluates to zero trivially.}
       &= \exp\left(\frac{-\left| \alpha \right|^{2}}{2}\right)
    \left[ a,e^{\alpha a^{\dagger}} \right] e^{-\bar{\alpha}a} \text{\quad where
    $ b = \alpha a^{\dagger} $} \\
\end{align}

\begin{align}
   \left[ a, e^{\alpha a^{\dagger}} \right] &= \left[ a, 1 + b +
   \frac{b^{2}}{2!} + \frac{b^{3}}{3!} + \ldots \right] \\
    &= [a,b] + [a,\frac{b^{2}}{2!}] + [a,\frac{b^{3}}{3!}] + \ldots \\
    &= \sum^{\infty}_{i=0}  \frac{\alpha^{i} [a,(a^{\dagger})^{i}]}{i!} \\
    %TODO: Prove the identity used here
    &= \sum^{\infty}_{i=1}  \frac{\alpha^{i} i (a^{\dagger})^{i-1}}{i!} \\
    &= \sum^{\infty}_{i=1}  \frac{\alpha^{i} (a^{\dagger})^{i-1}}{(i-1)!} \\
    &=  \alpha \sum^{\infty}_{i=1} \frac{\alpha^{i-1} (a^{\dagger})^{i-1}}{(i-1)!} \\
    &= \alpha \sum^{\infty}_{j=0} \frac{\alpha^{j} (a^{\dagger})^{j}}{j!} \\
    &= \alpha \sum^{\infty}_{j=0} \frac{\alpha^{j} (a^{\dagger})^{j}}{j!} \\
    &= \alpha \sum^{\infty}_{j=0} \frac{(\alpha a^{\dagger})^{j}}{j!} \\
    &= \alpha e^{\alpha a^{\dagger}}
\end{align}

Thus,
\[
   [a, D(\alpha)] =
   \alpha
   \exp\left(\frac{-\left| \alpha \right|^{2}}{2}\right)
   e^{\alpha a^{\dagger}}
   e^{-\bar{\alpha}a} =
   \alpha D(\alpha)
\]

Now, $ \left[ a, D(\alpha) \right] \ket{0} = \alpha \left( D(\alpha)
\ket{0} \right) $ from the above. However, $ \left[ a, D(\alpha) \right]
\ket{0} = (a D(\alpha) - D(\alpha) a) \ket{0}$, by definition of the
commutator. Since $ \alpha \ket{0} = 0 $ this expression reduces to $ \left[
a, D(\alpha) \right] = a D(\alpha) \ket{0} $. Thus, $ a D(\alpha) \ket{0} =
\alpha D(\alpha) \ket{0} $ and $ D(\alpha) \ket{0} $ is an eigenstate of $ a $
with eigenvalue $ \alpha $. This is exactly what we mean by the coherent state $
\ket{\alpha} $.
\end{homeworkSection}
\end{homeworkProblem}
