\begin{homeworkProblem}
\begin{homeworkSection}{(a)}
The Hamiltonian for a \textit{driven simple harmonic oscilator} is:
\begin{equation}\label{P2-H}
H=\frac{p^2}{2m}+\frac{1}{2}m\omega^2 x^2-xF(t)-pG(t)
\end{equation}
Canonical equations of motion reads:
\begin{align}
\dot{x}&=\pd{H(x,p,t)}{p}=\frac{p}{m}-G(t)\label{P2-1}\\
\dot{p}&=-\pd{H(x,p,t)}{x}=-m\omega^2 x+F(t)\label{P2-2}
\end{align} 
Combining \eqref{P2-1} and \eqref{P2-2} leads to the following differential equation for $x(t)$:
\begin{equation}
\ddot{x}=\frac{1}{m}\dot{p}-\frac{dG(t)}{dt}=-\omega^2 x+\frac{F(t)}{m}-\frac{dG(t)}{dt}
\end{equation}
\end{homeworkSection}
%-----b-------------------
\begin{homeworkSection}{(b)}
We define ladder operators like an unperturbed SHO:
\begin{equation}
a=\sqrt{\frac{m\omega}{2\hbar}}\left(x+\frac{ip}{m\omega}\right)\qquad
a^\dagger=\sqrt{\frac{m\omega}{2\hbar}}\left(x-\frac{ip}{m\omega}\right)
\end{equation}
$x$ and $p$ can be calculated in terms of $a$ and $a^\dagger$:
\begin{equation}\label{P2-3}
x=\sqrt{\frac{\hbar}{2m\omega}}\left(a+a^{\dagger}\right)\qquad
p=-im\omega\sqrt{\frac{\hbar}{2m\omega}}\left(a-a^{\dagger}\right)
\end{equation}
The commutation relation between $a$ and $a^\dagger$ is:
\begin{equation}
[a,a^\dagger]=\frac{m\omega}{2\hbar}\left[x+\frac{ip}{m\omega},x-\frac{ip}{m\omega}\right]=\frac{1}{i\hbar}[x,p]=1
\end{equation}
First two terms in the right hand side of \eqref{P2-H} can be simply replaced by $\hbar\omega(a^\dagger a+1/2)$ and for the other terms we use \eqref{P2-3} so we get:
\begin{equation}\label{P2-H2}
H=\hbar\omega\left(a^\dagger a+\frac{1}{2}\right)-\sqrt{\frac{\hbar}{2m\omega}}\left\{F(t)+im\omega G(t)\right\} a-\sqrt{\frac{\hbar}{2m\omega}}\left\{F(t)-im\omega G(t)\right\} a^\dagger
\end{equation} 
\end{homeworkSection}
%--------------------c----------------------------
\begin{homeworkSection}{(c)} 
 In the Heisenberg picture operators are time dependent and equations of motion are simply:
\begin{align}
\frac{da}{dt}&=\frac{1}{i\hbar}[a,H]+\pd{a}{t}\\
\frac{da^\dagger}{dt}&=\frac{1}{i\hbar}[a^\dagger,H]+\pd{a^\dagger}{t}
\end{align}
By inserting the Hamiltonian from \eqref{P2-H2} and using $a$ and $a^\dagger$  commutation relation we obtain:
\begin{align}
\frac{da}{dt}&=-i\omega [a,a^\dagger a+\frac{1}{2}]-\sqrt{\frac{\hbar}{2m\omega}}\left\{F(t)-im\omega G(t)\right\}=-i\omega a-\sqrt{\frac{\hbar}{2m\omega}}\left\{F(t)-im\omega G(t)\right\}\label{P2-400}\\
\frac{da^\dagger}{dt}&=+i\omega [a^\dagger,a^\dagger a+\frac{1}{2}]-\sqrt{\frac{\hbar}{2m\omega}}\left\{F(t)+im\omega G(t)\right\}=i\omega a -\sqrt{\frac{\hbar}{2m\omega}}\left\{F(t)+im\omega G(t)\right\}\label{P2-401}
\end{align}
To solve these differential equations we use a new operator which is defined by:
\begin{equation}
Q=a e^{i\omega t}
\end{equation}
Using this definition \eqref{P2-400} and \eqref{P2-401} are translated as 
\begin{align}
\frac{da}{dt}&=-i\omega Q e^{-i\omega t}+\frac{dQ}{dt}e^{-i\omega t}=-i\omega Q e^{-i\omega t}-\sqrt{\frac{\hbar}{2m\omega}}\left\{F(t)-im\omega G(t)\right\}\\
\frac{da^\dagger}{dt}&=+i\omega Q^\dagger e^{i\omega t}+\frac{dQ^\dagger}{dt}e^{+i\omega t}=+i\omega Q^\dagger e^{i\omega t}-\sqrt{\frac{\hbar}{2m\omega}}\left\{F(t)+im\omega G(t)\right\}
\end{align}
So simply we get:
\begin{equation}
Q(t)=Q(0)-\sqrt{\frac{\hbar}{2m\omega}}\int_{t'=0}^t \left\{F(t')-im\omega G(t')\right\}e^{i\omega t'}dt'
\end{equation}
therefore
\begin{align}
a(t)&=a(0)e^{-i\omega t}-\sqrt{\frac{\hbar}{2m\omega}}e^{-i\omega t}\int_{t'=0}^t \left\{F(t')-im\omega G(t')\right\}e^{i\omega t'}dt'\\
a^\dagger(t)&=a^\dagger(0)e^{i\omega t}-\sqrt{\frac{\hbar}{2m\omega}}e^{i\omega t}\int_{t'=0}^t \left\{F(t')+im\omega G(t')\right\}e^{-i\omega t'}dt'
\end{align}
\end{homeworkSection}
\begin{homeworkSection}{(d)}
It's assumed that $F(t)$ and $G(t)$ just act in $0<t<T$ and the initial state is the ground state of the original Hamiltonian. To find the final state at $t=T$ we use Sch\"odinger picture. We try to find time evolution operator which can predict state vector in an arbitary time. From schr\"odinger equation we have:
\begin{equation}\label{P2-500}
i\hbar\pd{U(t,0)}{t}=HU(t,0)
\end{equation}
In above equation $U(t,0)$ is the time evolution operator statevector at a given time is:
\begin{equation}
\ket{\Psi(t)}=U(t,0)\ket{\Psi(t=0)}
\end{equation} 
First note that:
\begin{equation}
[H(t_1),H(t_2)]=[H_0-xF(t_1)-pG(t_1),H_0-xF(t_2)-pG(t_2)]\neq 0
\end{equation}
Since Hamiltonian in two different time are not commuative we can not solve \eqref{P2-500} by direct integartion similar to the analytic function in a simple commutative complex space. Instead we have to use \textit{Dyson series} \cite{sakurai}. In this case time evolution operator is:
\begin{equation}
U(t,0)=1+\sum\limits_{n=1}^{\infty}\left(\frac{-i}{\hbar}\right)^n\int_0^{t}dt_1\int_0^{t_1}dt_2\cdots\int_0^{t_{n-1}}dt_nH(t_1)H(t_2)\cdots H(t_n)
\end{equation}
The desired quantity is the correlation of the state $\ket{n}$ and the evolved wavefunction at $t=T$. 
\begin{equation}
p(n)=\abs{\bracket{n}{\Psi(T)}}^2=\abs{\bracket{n}{\Psi(t)}}^2\qquad\text{for $t>T$} 
\end{equation} 
We may calculate $U_{n0}$ to get $p(n)$:
\begin{equation}
U_{n0}(T,0)=\delta_{n0}+\sum\limits_{m=1}^{\infty}\left(\frac{-i}{\hbar}\right)^m\int_0^{T}dt_1\int_0^{t_1}dt_2\cdots\int_0^{t_{m-1}}dt_m\bra{n}H(t_1)H(t_2)\cdots H(t_m)\ket{0}
\end{equation}
If we insert unity operator between H's we arrive at:
\begin{multline}\label{P2-bbb}
U_{n0}(T,0)=\delta_{n0}+\\
\sum\limits_{m=1}^{\infty}\sum\limits_{k_1,k_2,\cdots}\left(\frac{-i}{\hbar}\right)^m\int_0^{T}dt_1\int_0^{t_1}dt_2\cdots\int_0^{t_{m-1}}dt_m\bra{n}H(t_1)\ket{k_1}\bra{k_1}H(t_2)\ket{k_2}\cdots \bra{k_{m-1}}H(t_m)\ket{0}
\end{multline}
Please note that $H$ connects contiguous states , i.e. the Hamiltonian at any instanse of time can just connect  $\ket{i}$ to $\ket{i}$ , $\ket{i-1}$ and $\ket{i+1}$. This statement means that we need at least $n$ H's to get a nonzero corrlation in \eqref{P2-bbb}. So the first n terms in the summation are zero so:
 \begin{multline}\label{P2-bbb}
U_{n0}(T,0)=\delta_{n0}+\\
\sum\limits_{m=n}^{\infty}\sum\limits_{k_1,k_2,\cdots}\left(\frac{-i}{\hbar}\right)^m\int_0^{T}dt_1\int_0^{t_1}dt_2\cdots\int_0^{t_{m-1}}dt_m\bra{n}H(t_1)\ket{k_1}\bra{k_1}H(t_2)\ket{k_2}\cdots \bra{k_{m-1}}H(t_m)\ket{0}
\end{multline}
The matrix elements of $H(t)$ can be explicitly calculated through the use of \eqref{P2-H2} :
\begin{equation}
\bra{k}H(t)\ket{l}=\hbar\omega\delta{kl}-\sqrt{\frac{l\hbar}{2m\omega}}\left\{F(t)+im\omega G(t)\right\}\delta_{k,l-1}-\sqrt{\frac{(l+1)\hbar}{2m\omega}}\left\{F(t)-im\omega G(t)\right\}\delta_{k,l+1}
\end{equation}
\end{homeworkSection}
\end{homeworkProblem}